AlgoLib.lean
@@ -91,5 +91,6 @@ import AlgoLib.Experimental.RAM.Tests.Algorithms
 import AlgoLib.Experimental.RAM.Tests.Paper
 import AlgoLib.Experimental.RAM.Tests.PaperAxioms
 import AlgoLib.Experimental.RAM.Tests.Methods
+import AlgoLib.Experimental.RAM.Prototype.FrameworkTests
 import AlgoLib.Experimental.RAM.Prototype.Tests
 import AlgoLib.Experimental.RAM.Prototype.Axioms
